Rename mk of ghost_well_formed to mk_ghost_well_formed

src/proof/apimodel.v
@@ -142,7 +142,7 @@ Proof.
 Qed.
 
 Record ghost_well_formed (used_uid: gset go_string) (abs_state: gmap KKey.t PureKObject.t) (children: gmap KKey.t (gset KKey.t)) (fresh_keys: gset KKey.t) : Prop :=
-mk {
+mk_ghost_well_formed {
   Habs_state_well_formed: (∀ k obj, abs_state !! k = Some obj → PureKObject.agree_with_key obj k ∧ PureKObject.well_formed obj);
   Hparents_exist: (dom children = dom abs_state);
   Hchildren_exist : (∀ k s, children !! k = Some s → s ⊆ dom abs_state);
